Start with urelements

src/Set_Semantics.thy
@@ -1,11 +1,11 @@
 theory Set_Semantics
-  imports Logic ZFC_Extras "HOL-Library.Adhoc_Overloading"
+  imports Logic ZFC_Extras "HOL-Library.Adhoc_Overloading" "HOL-Library.Monad_Syntax"
 begin
 
 section \<open>Syntax and Semantics\<close>
 
 datatype (vars_term: 'a) pset_term = 
-  Empty (\<open>\<emptyset>\<close>)| is_Var: Var 'a |
+  Empty nat (\<open>\<emptyset> _\<close>) | is_Var: Var 'a |
   Union "'a pset_term" "'a pset_term" (infixr \<open>\<squnion>\<^sub>s\<close> 60) |
   Inter "'a pset_term" "'a pset_term" (infixr \<open>\<sqinter>\<^sub>s\<close> 70) |
   Diff "'a pset_term" "'a pset_term"  (infixl \<open>-\<^sub>s\<close> 80) |
@@ -22,7 +22,7 @@ type_synonym 'a pset_fm = "'a pset_atom fm"
 type_synonym 'a branch = "'a pset_fm list"
 
 fun I\<^sub>s\<^sub>t :: "('a \<Rightarrow> V) \<Rightarrow> 'a pset_term \<Rightarrow> V" where
-  "I\<^sub>s\<^sub>t v \<emptyset> = 0"
+  "I\<^sub>s\<^sub>t v (\<emptyset> _) = 0"
 | "I\<^sub>s\<^sub>t v (Var x) = v x"
 | "I\<^sub>s\<^sub>t v (s1 \<squnion>\<^sub>s s2) = I\<^sub>s\<^sub>t v s1 \<squnion> I\<^sub>s\<^sub>t v s2"
 | "I\<^sub>s\<^sub>t v (s1 \<sqinter>\<^sub>s s2) = I\<^sub>s\<^sub>t v s1 \<sqinter> I\<^sub>s\<^sub>t v s2"
@@ -124,7 +124,7 @@ lemma subfmsD:
 subsection \<open>Subterms\<close>
 
 fun subterms_term :: "'a pset_term \<Rightarrow> 'a pset_term set"  where
-  "subterms_term \<emptyset> = {\<emptyset>}"
+  "subterms_term (\<emptyset> n) = {\<emptyset> n}"
 | "subterms_term (Var i) = {Var i}"
 | "subterms_term (t1 \<squnion>\<^sub>s t2) = {t1 \<squnion>\<^sub>s t2} \<union> subterms_term t1 \<union> subterms_term t2"
 | "subterms_term (t1 \<sqinter>\<^sub>s t2) = {t1 \<sqinter>\<^sub>s t2} \<union> subterms_term t1 \<union> subterms_term t2"
@@ -375,5 +375,52 @@ lemma subterms_atom_nonempty[simp]: "subterms_atom l \<noteq> {}"
 
 lemma subterms_fm_nonempty[simp]: "subterms_fm \<phi> \<noteq> {}"
   by (induction \<phi>) auto
+
+section \<open>Typing\<close>
+
+term "x :: 'a option"
+
+fun type_term :: "('a \<Rightarrow> nat) \<Rightarrow> 'a pset_term \<Rightarrow> nat option" where
+    "type_term _ (\<emptyset> n) = Some (Suc n)"
+  | "type_term v (Var x) = Some (v x)"
+  | "type_term v (Single t) = map_option Suc (type_term v t)"
+  | "type_term v (s \<squnion>\<^sub>s t) = do {
+                            ts <- type_term v s;
+                            tt <- type_term v t;
+                            if tt \<noteq> 0 \<and> tt = ts then Some tt else None
+                          }"
+  | "type_term v (s \<sqinter>\<^sub>s t) = do {
+                            ts <- type_term v s;
+                            tt <- type_term v t;
+                            if tt \<noteq> 0 \<and> tt = ts then Some tt else None
+                          }"
+  | "type_term v (s -\<^sub>s t) = do {
+                            ts <- type_term v s;
+                            tt <- type_term v t;
+                            if tt \<noteq> 0 \<and> tt = ts then Some tt else None
+                          }"
+
+consts types :: "('a \<Rightarrow> nat) \<Rightarrow> 'b \<Rightarrow> bool" ("_ \<turnstile> _" 45)
+
+inductive types_pset_atom :: "('a \<Rightarrow> nat) \<Rightarrow> 'a pset_atom \<Rightarrow> bool" where
+  "\<lbrakk> type_term v s = Some n; type_term v t = Some n \<rbrakk> \<Longrightarrow> types_pset_atom v (s =\<^sub>s t)"
+| "\<lbrakk> type_term v s = Some n; type_term v t = Some (Suc n) \<rbrakk> \<Longrightarrow> types_pset_atom v (s \<in>\<^sub>s t)"
+
+adhoc_overloading types types_pset_atom
+
+definition types_pset_fm :: "('a \<Rightarrow> nat) \<Rightarrow> 'a pset_fm \<Rightarrow> bool" where
+  "types_pset_fm v \<phi> \<equiv> (\<forall>a \<in> atoms \<phi>. v \<turnstile> a)"
+
+adhoc_overloading types types_pset_fm
+
+definition urelem :: "'a pset_fm \<Rightarrow> 'a pset_term \<Rightarrow> bool" where
+  "urelem \<phi> t \<equiv> (\<exists>v. v \<turnstile> \<phi> \<and> type_term v t = Some 0)"
+
+lemma is_Var_if_type_term_0: "type_term v t = Some 0 \<Longrightarrow> is_Var t"
+  by (induction t) (auto split: if_splits Option.bind_splits)
+
+lemma is_Var_if_urelem: "urelem \<phi> t \<Longrightarrow> is_Var t"
+  unfolding urelem_def using is_Var_if_type_term_0 by blast
+
 
 end
